---
title: '$\alpha$-limit and $\omega$-limit of $S^1$'
date: 2023-09-20
tags:
  - learning notes
  - dynamic system
---

In this note, we will talk about the dynamic system of homeomorphism on $S^1$.

## $\alpha$-limit and $\omega$-limit of $S^1$

$\rho: S^1 \to S^1$ orient-preserve homeomophism.
We can define **$\omega$-limit** and **$\alpha$-limit** sets of $x \in S^1$:
$$
\omega(x) :=\{y \in S^1: \exists m_i \to +\infty \text{ s.t. } \rho^{m_i}(x) \to y \text{ as }i\to+\infty\}
$$
$$
\alpha(x) :=\{y \in S^1: \exists m_i \to -\infty \text{ s.t. } \rho^{m_i}(x) \to y \text{ as }i\to+\infty\}
$$

**Example.** $\rho = \mathrm R_\alpha, \alpha \in \mathbb R - \mathbb Q \Rightarrow \omega(x)=S^1,\alpha(x)=s^1\forall x \in S^1$


>**Prop.** 
>	If $\rho(f) \in \mathbb R - \mathbb Q$, then $\omega(x)=\omega(y)\forall x \not = y \in S^1$


To prove this proposition, we need a lemma below.

>**Lemma.**
>	Assume $\rho(f) \in \mathbb R - \mathbb Q$. Let $x,z \in S^1, m > n \in \mathbb N$, and let $I = [\rho^n(x), \rho^m(x)]\subset S^1$.
>	Then, $\exists k \in \mathbb N^*$ s.t. $\rho^k(z)\in I$.

**proof of lemma.**
	The intervals $\rho^{-k(m-n)}(I)$ and $\rho^{-(k-1)(m-n)}(I)$ have a common boundary.
	Then, we have  two case:
	case1: $\sum_{k=1}^\infty l(\rho^{-k(m-n)}(I))$ converge
		That is, $\rho^{-k(m-n)}(I)$ converge to one point $y \in S^1$.
		Since $\rho^{-(m-n)}(y) = y$, implies $y$ is a periodic point of $\rho$, an contraction.
	case2: $\sum_{k=1}^\infty l(\rho^{-k(m-n)}(I))$ not converge
		Then, $S^1$ will be covered finite of $\{\rho^{-k(m-n)}(I)\}$.
		That is, there exist $k_0 \in \mathbb N$ s.t. $z_0 \in \rho^{-k(m-n)}(I)$.
		Hence, $\rho^{k(m-n)}(z) \in I$.


**proof of thm.**
	$\rho (f) \in \mathbb R - \mathbb Q$, $x \not = y \in S^1$
	we want to show that $\omega (x) = \omega(y)$
	First, we choose $x_0 \in \omega(x)$, then $\exists m_i \to +\infty$ s.t. $\rho^{m_i}(x) \to x_0$.
	By the lemma, $\exists k_i \in \mathbb N$ s.t. $\rho^{k_i}(y) \in [\rho^{n_i}(x), \rho^{n_i + 1}(x)]$.
	Without losing generality, we can choose $k_{i+1} > k_i, \forall i$ so that $k_i \to +\infty$ as $i\to +\infty$.
	Since $\rho^{n_i}(x) \to x_0$, we obtain $\rho^{k_i}(y) \to x_0$.
	Then, $x_0 \in \omega(y)$ implies $\omega(x) \subset \omega(y)$.
	By summetry, we also have $\omega(y) \subset \omega(x)$.
	Hence, $\omega(x) = \omega(y)$.